coq/Proofs/Revocation.v
@@ -40,12 +40,10 @@ End DummyTagDefs.
 
 Module RevocationProofs.
 
-  Fixpoint remove_PNVI (x:cerb_switches_t) : cerb_switches_t :=
-    match x with
-    | nil => empty_set _
-    | SW_PNVI _ :: xs => remove_PNVI xs
-    | x :: xs => x :: remove_PNVI xs
-    end.
+  (* --- Memory models instantiated with and without PNVI --- *)
+
+  Definition remove_PNVI: cerb_switches_t -> cerb_switches_t :=
+    List.filter (fun s => negb (is_PNVI_switch s)).
 
   (* Removes all other PNVI flavours *)
   Module WithoutPNVISwitches.
@@ -67,8 +65,95 @@ Module RevocationProofs.
     Include CheriMemoryImpl(Capability_GS)(MorelloImpl)(DummyTagDefs)(WithPNVISwitches).
   End CheriMemoryWithPNVI.
 
-(*  Theorem foo:
+  (* --- Equality predicates for types used in Memory Models --- *)
+
+  Definition function_pointer_eq
+    (a:CheriMemoryWithPNVI.function_pointer)
+    (b:CheriMemoryWithoutPNVI.function_pointer)
+    :=
+    match a,b with
+    | CheriMemoryWithPNVI.FP_valid s1, CheriMemoryWithoutPNVI.FP_valid s2 => s1 = s2
+    | CheriMemoryWithPNVI.FP_invalid c1, CheriMemoryWithoutPNVI.FP_invalid c2 => c1 = c2
+    | _, _ => False
+    end.
+
+  Definition pointer_value_base_eq
+    (a:CheriMemoryWithPNVI.pointer_value_base)
+    (b:CheriMemoryWithoutPNVI.pointer_value_base)
+    :=
+    match a,b with
+    | CheriMemoryWithPNVI.PVfunction f1, CheriMemoryWithoutPNVI.PVfunction f2 => function_pointer_eq f1 f2
+    | CheriMemoryWithPNVI.PVconcrete c1, CheriMemoryWithoutPNVI.PVconcrete c2 => c1 = c2
+    | _, _ => False
+    end.
+
+  Definition provenance_eq
+    (a:CheriMemoryWithPNVI.provenance)
+    (b:CheriMemoryWithoutPNVI.provenance) : Prop
+    :=
+    match a,b with
+    | CheriMemoryWithPNVI.Prov_disabled, CheriMemoryWithoutPNVI.Prov_disabled => True
+    | CheriMemoryWithPNVI.Prov_none, CheriMemoryWithoutPNVI.Prov_none => True
+    | CheriMemoryWithPNVI.Prov_some id1, CheriMemoryWithoutPNVI.Prov_some id2 =>
+        id1 = id2
+    | CheriMemoryWithPNVI.Prov_symbolic sid1, CheriMemoryWithoutPNVI.Prov_symbolic sid2 =>
+        sid1 = sid2
+    | CheriMemoryWithPNVI.Prov_device, CheriMemoryWithoutPNVI.Prov_device => True
+    | _, _ => False
+    end.
+
+  (* Compare pointer values without taking provenance into account *)
+  Definition pointer_value_eq
+    (a:CheriMemoryWithPNVI.pointer_value)
+    (b:CheriMemoryWithoutPNVI.pointer_value) : Prop
+    :=
+    match a,b with
+    | CheriMemoryWithPNVI.PV p1 b1, CheriMemoryWithoutPNVI.PV p2 b2 =>
+        (* provenance_eq p1 p2 /\ *) pointer_value_base_eq b1 b2
+    end.
+
+  Lemma is_PNVI_WithPNVI:
+    is_PNVI (WithPNVISwitches.get_switches tt) = true.
+  Proof.
+    unfold WithPNVISwitches.get_switches.
+    remember (abst_get_switches tt) as l.
+    apply existsb_exists.
+    exists (SW_PNVI AE_UDI).
+    split.
+    2:reflexivity.
+    apply set_add_iff.
+    left.
+    reflexivity.
+  Qed.
+
+  Lemma is_PNVI_WithoutPNVI:
+    is_PNVI (WithoutPNVISwitches.get_switches tt) = false.
+  Proof.
+    unfold WithoutPNVISwitches.get_switches.
+    remember (abst_get_switches tt) as l.
+    unfold is_PNVI, remove_PNVI in *.
+    apply Bool.not_true_is_false.
+    intros E.
+    apply Bool.Is_true_eq_left in E.
+    apply list.existb_True in E.
+    apply Exists_exists in E.
+    destruct E as [x [H0 H1]].
+    apply filter_In in H0.
+    destruct H0 as [H2 H3].
+    apply Bool.negb_true_iff in H3.
+    rewrite H3 in H1.
+    inversion H1.
+  Qed.
+
+  (* --- Lemmas about memory models --- *)
+
+  Theorem null_ptrval_same:
     forall t,
-      CheriMemoryWithoutPNVI.null_ptrval t <> CheriMemoryWithPNVI.null_ptrval t.
-*)
+      pointer_value_eq
+        (CheriMemoryWithPNVI.null_ptrval t)
+        (CheriMemoryWithoutPNVI.null_ptrval t).
+  Proof.
+    reflexivity.
+  Qed.
+
 End RevocationProofs.
